case_study/RiscvPmp/FemtoKernel.v
@@ -215,7 +215,6 @@ Module inv := invariants.
     Example femtokernel_init' (init_start : N) (handler_start : N) (adv_start : N) : list AnnotInstr :=
       resolve_ASM (femtokernel_init_asm handler_start adv_start) init_start.
 
-    (* fdu *)
     Example femtokernel_mmio_handler_asm_block0 (mmio_handler_start_block2 : N) (data_start : N) : list ASM :=
       [
         (* ITYPE bv.one zero t1 RISCV_ADDI (* t1 <- 1 *) *)
@@ -369,7 +368,6 @@ Module inv := invariants.
       asn_mmio_trace_state_inv
     .
 
-    (* fdu *)
     Example femtokernel_handler_post_block0 : Assertion ["a" :: ty_xlenbits; "an"::ty_xlenbits] :=
       (term_var "a" = term_val ty_word (bv.of_N handler_addr)) ∗
       (term_unop uop.unsigned (term_var "a") + term_val ty.int (Z.of_N (adv_addr - handler_addr)) < term_val ty.int (Z.of_N maxAddr))%asn ∗
@@ -377,23 +375,26 @@ Module inv := invariants.
       (mtvec ↦ term_val ty_word (bv.of_N handler_addr)) ∗
       (∃ "cause", mcause ↦ term_var "cause") ∗
       (∃ "epc", mepc ↦ term_var "epc") ∗
-      (∃ "v", (term_var "a" +ᵇ term_val ty_xlenbits (bv.of_N mmio_handler_size)) ↦ᵢ term_var "v") ∗
+      (* (∃ "v", (term_var "a" +ᵇ term_val ty_xlenbits (bv.of_N mmio_handler_size)) ↦ᵢ term_var "v") ∗ *)
       asn_regs_ptsto_excl [5] ∗
       cur_privilege ↦ term_val ty_privilege Machine ∗
       asn_pmp_entries (term_list (asn_femto_pmpentries (term_var "a" -ᵇ term_val ty_xlenbits (bv.of_N handler_addr)))) ∗ (* Different handler sizes cause different entries *)
-      (∃ "w", ∃ "s",
-            ((asn.chunk (chunk_ptsreg x5 (term_var "w"))) ∗
-            (asn.or
-               ( (* we reach block1 and t0 contains a value that satisfies the mmio_state protocol *)
-                 (asn.chunk (chunk_user (mmio_state_prot bytes_per_word) [(term_var "w"); (term_var "s")])) ∗
-                 (asn_mmio_state_pred (term_var "s")) ∗
-                 (term_var "an" = term_val ty_word (bv.of_N mmio_handler_addr_block1))
-               )
-               ( (* we jump to block2 essentially skipping the write *)
-                 (asn_mmio_state_pred (term_var "s")) ∗
-                 (term_var "an" = term_val ty_word (bv.of_N mmio_handler_addr_block2))
-               )
-      ))) ∗
+      (∃ "oldvalue", ∃ "newvalue", ∃ "s",
+          asn.sep
+           (    (asn.chunk (chunk_ptsreg x5 (term_var "newvalue")))
+              ∗ (asn_mmio_state_pred (term_var "s"))
+              ∗ (term_var "a" +ᵇ term_val ty_xlenbits (bv.of_N mmio_handler_size)) ↦ᵢ (term_var "oldvalue")
+           )
+           (asn.or
+             (
+               (asn.formula (formula_user (mmio_state_prot bytes_per_word) [term_var "newvalue"; term_var "s"])) ∗ 
+               (term_var "an" = term_val ty_word (bv.of_N mmio_handler_addr_block1))
+             )
+             (
+               (term_var "an" = term_val ty_word (bv.of_N mmio_handler_addr_block2))
+             )
+          )
+      ) ∗
       asn_mmio_trace_state_inv.
 
   Example femtokernel_handler_pre_block1 : Assertion ["a" :: ty_xlenbits] :=
@@ -505,38 +506,39 @@ Import Erasure.notations.
 (* for debugging *)
 Set Printing Depth 200.
 Eval vm_compute in vc__femtohandler_block0.
-(* fdu *)
     (* Prove that the verification condition that Katamaran creates for this block holds.
        I.e. we're just proving the verification condition for block0. *)
     Import Erasure.notations.
     Lemma sat__femtohandler_block0 : safeE (vc__femtohandler_block0).
     Proof.
       vm_compute.
-      constructor; cbn. unfold bv.sext'. intros. destruct (bv.msb v).
-      -  (* courtesy of Dominique Devriese *)
-         destruct (bv.appView 1 _ v).
-         change (@bv.mk 32 1 I) with (@bv.app 1 31 [bv 0x1] bv.zero) in H.
-         change (@bv.land 32) with (@bv.land (1 + 31)) in H.
-         rewrite bv.land_app in H.
-         apply (f_equal (bv.take 1)) in H.
-         rewrite !bv.take_app in H.
-         now rewrite bv.land_ones_r in H.
-      -  unfold bv.take. destruct (bv.appView 1 _ v).
-         destr
-           uct xs. destruct bin.
-         -- simpl in *. rewrite <- bv.of_N_wf. auto.
-         -- simpl in *. destruct p; inversion i.
-            destruct H.
-            rewrite <- bv.of_N_wf.
-            rewrite bv.of_N_one. simpl.
-            change (@bv.mk 32 1 I) with (@bv.app 1 31 [bv 0x1] bv.zero).
-            change (@bv.land 32) with (@bv.land (1 + 31)).
-            rewrite bv.land_app.
-            rewrite bv.land_zero_r.
-            change ([bv 0x1] : bv 1) with (bv.ones 1).
-            rewrite bv.land_ones_r.
-            reflexivity.
-    Qed.
+      constructor; cbn. intros. split; auto.
+      unfold Mmio_state_prot. intros. admit.
+    Admitted.
+    (*   -  (* courtesy of Dominique Devriese *) *)
+    (*     intros. *)
+    (*      destruct (bv.appView 1 _ v). *)
+    (*      change (@bv.mk 32 1 I) with (@bv.app 1 31 [bv 0x1] bv.zero) in H. *)
+    (*      change (@bv.land 32) with (@bv.land (1 + 31)) in H. *)
+    (*      rewrite bv.land_app in H. *)
+    (*      apply (f_equal (bv.take 1)) in H. *)
+    (*      rewrite !bv.take_app in H. *)
+    (*      now rewrite bv.land_ones_r in H. *)
+    (*   -  unfold bv.take. destruct (bv.appView 1 _ v). *)
+    (*      destruct xs. destruct bin. *)
+    (*      -- simpl in *. rewrite <- bv.of_N_wf. auto. *)
+    (*      -- simpl in *. destruct p; inversion i. *)
+    (*         destruct H. *)
+    (*         rewrite <- bv.of_N_wf. *)
+    (*         rewrite bv.of_N_one. simpl. *)
+    (*         change (@bv.mk 32 1 I) with (@bv.app 1 31 [bv 0x1] bv.zero). *)
+    (*         change (@bv.land 32) with (@bv.land (1 + 31)). *)
+    (*         rewrite bv.land_app. *)
+    (*         rewrite bv.land_zero_r. *)
+    (*         change ([bv 0x1] : bv 1) with (bv.ones 1). *)
+    (*         rewrite bv.land_ones_r. *)
+    (*         reflexivity. *)
+    (* Qed. *)
 
     Lemma sat__femtohandler_block1 : safeE (vc__femtohandler_block1).
     Proof.
